still in the process of applying laws

InsertionSort.dfy
@@ -4,7 +4,7 @@ method PairInsertionSort(a: array<int>)
 	ensures multiset(a[..]) == multiset(old(a[..]))
 	modifies a
 {
-	//introdue local variable + leading assignemnt + weaken precondition
+	//introdue local variable + introduce logical constant + weaken precondition
 	ghost var A := multiset(old(a[..]));
 	PairInsertionSort1(a,A);
 }
@@ -25,9 +25,9 @@ method initIJ(ghost a: array<int>, j0: int,i0:nat, ghost A: multiset<int>) retur
 	ensures InvPair(a[..],j,i,A)
 	modifies a
 	{
+		j,i:=j0,i0;
 		//assignment
 		LemmainitIJ(a,j,i,A);
-		j,i:=j0,i0;
 		j,i:=-1,0;
 	}
 lemma LemmainitIJ( a: array<int>, j: int,i:nat,  A: multiset<int>)
@@ -81,44 +81,156 @@ method MainLoopBody(a: array<int>, j0: int,i0:nat,x0:int, y0:int, ghost A: multi
 	ensures InvPair(a[..],j,i,A) && (a.Length-i)< (a.Length-i0)
 	modifies a
 {
+	//sequential composition+contract frame
 	j,i,x,y:=j0,i0,x0,y0;
-	x,y:=a[i],a[i+1];
-		if x<y {
-			x,y:=y,x;
-		}
-		else{
-
-		} 
-		j:= i-1;
-		while j>=0 && a[j]>x
-			invariant Inv2Pair(a[..],j,i,x,y,A)
-			decreases j
-			{
-				SwapPair(a,j+2,j,A);
-				j:=j-1;
-			}
-		if a[j+2]!=x{
-			LemmaMidswap(a[..],j,i,x,y,A);
-			SwapPair(a,j+2,j+1,A);
-		}	
-		else{
-			LemmaMidNoswap(a[..],j,i,x,y,A);
-		}
-		
-		
-		while j>=0 && a[j] > y
-			invariant Inv3Pair(a[..],j,i,x,y,A)
-			decreases j
-			{
-				SwapPair(a,j+1,j,A);
-				j:=j-1;
-			}
-		
-		i:=i+2;	
+	j,x,y:=preFirstInnerLoop(a,j,i,x,y,A);
+	j,i,x,y:=MainLoopBody2(a,j,i,x,y,A);
 }
+
+method preFirstInnerLoop(a: array<int>, j0: int,i:nat,x0:int, y0:int, ghost A: multiset<int>) returns (j:int,x:int,y:int)
+	requires InvPair(a[..],j0,i,A) && GuardMainLoop(a,i)
+	ensures Inv2Pair(a[..],j,i,x,y,A)
+	{
+		j,x,y:=j0,x0,y0;
+		//leading assignemnt+following assignment+contract frame+weaken precondition
+		x,y:=a[i],a[i+1];
+		x,y:=adjustXY(a,j,i,x,y,A);
+		j:= i-1;
+	}
+method adjustXY(a: array<int>, j: int,i:nat,x0:int, y0:int, ghost A: multiset<int>) returns (x:int,y:int)
+	requires InvPair(a[..],j,i,A) && GuardMainLoop(a,i) && x0==a[i]&&y0==a[i+1]
+	ensures Inv2Pair(a[..],i-1,i,x,y,A)
+	{
+		x,y:=x0,y0;
+		//alternaion
+		if x<y {
+			x,y:=xSmaller(a,j,i,x,y,A);
+		}
+		else{
+			LemmaxGreaterOrEqual(a,j,i,x,y,A);
+		} 
+	}
+method xSmaller (a: array<int>, j: int,i:nat,x0:int, y0:int, ghost A: multiset<int>) returns (x:int,y:int)
+	requires InvPair(a[..],j,i,A) && GuardMainLoop(a,i) && x0==a[i]&&y0==a[i+1] && x0<y0
+	ensures Inv2Pair(a[..],i-1,i,x,y,A)
+
+	{
+		x,y:=x0,y0;
+		//assignment
+		x,y:=y,x;
+	}
+
+lemma LemmaxSmaller (a: array<int>, j: int,i:nat,x:int, y:int,  A: multiset<int>)
+	requires InvPair(a[..],j,i,A) && GuardMainLoop(a,i) && x==a[i]&&y==a[i+1] && x<y
+	ensures Inv2Pair(a[..],i-1,i,y,x,A)
+
+lemma LemmaxGreaterOrEqual (a: array<int>, j: int,i:nat,x:int, y:int,  A: multiset<int>)
+	requires InvPair(a[..],j,i,A) && GuardMainLoop(a,i) && x==a[i]&&y==a[i+1] && x>=y
+	ensures Inv2Pair(a[..],i-1,i,x,y,A)
+
+method MainLoopBody2(a: array<int>, j0: int,i0:nat,x0:int, y0:int, ghost A: multiset<int>) returns (j: int,i:nat,x:int,y:int)
+	requires Inv2Pair(a[..],j0,i0,x0,y0,A)
+	ensures InvPair(a[..],j,i,A) && (a.Length-i)< (a.Length-i0)
+	modifies a
+{
+	//sequential composition+contract frame
+	j,i,x,y:=j0,i0,x0,y0;
+	j:=firstInnerLoop(a,j,i,x,y,A);
+	j,i,x,y:=MainLoopBody3(a,j,i,x,y,A);
+}
+
+method firstInnerLoop(a: array<int>, j0: int,i:nat,x:int, y:int, ghost A: multiset<int>) returns (j: int)
+	requires Inv2Pair(a[..],j0,i,x,y,A)
+	ensures Inv2Pair(a[..],j,i,x,y,A) && !GuardSecondLoop(a,j,x)
+	modifies a
+	{
+		j:=j0;
+		//iteration
+		while GuardSecondLoop(a,j,x)
+		invariant Inv2Pair(a[..],j,i,x,y,A)
+		decreases j
+		{
+			j:=firstInnerLoopBody(a,j,i,x,y,A);
+		}
+	}
+
+method firstInnerLoopBody(a: array<int>, j0: int,i:nat,x:int, y:int, ghost A: multiset<int>) returns (j: int)
+	requires Inv2Pair(a[..],j0,i,x,y,A) && GuardSecondLoop(a,j0,x)
+	ensures Inv2Pair(a[..],j,i,x,y,A) && j<j0
+	modifies a
+
+	{
+		j:=j0;
+		//following assignment+contract frame
+		SwapFirstInner(a,j,i,x,y,A);
+		j:=j-1;
+	}
+method {:verify true} SwapFirstInner(a: array<int>, j:int, i: nat,x:int,y:int ,ghost A: multiset<int>) 
+	requires Inv2Pair(a[..], j, i,x, y, A) && GuardSecondLoop(a,j,x)
+	ensures Inv2Pair(a[..], j-1, i,x, y, A) // && j-1 < j
+	modifies a
+{
+	// assignment
+	LemmaSwapFirstInner(a, j, i, x, y, A);
+	a[j+2], a[j] := a[j], a[j+2];
+}
+
+lemma LemmaSwapFirstInner(a: array<int>, j: int, i: nat,x:int,y:int, A: multiset<int>)
+	requires Inv2Pair(a[..], j, i, x, y, A) && GuardSecondLoop(a,j,x)
+	ensures Inv2Pair(a[..][j := a[j+2]][j+2 := a[j]], j-1, i, x, y, A) 
+{}
+
+method MainLoopBody3(a: array<int>, j0: int,i0:nat,x0:int, y0:int, ghost A: multiset<int>) returns (j: int,i:nat,x:int,y:int)
+	requires Inv2Pair(a[..],j0,i0,x0,y0,A) && !GuardSecondLoop(a,j0,x0)
+	ensures InvPair(a[..],j,i,A) && (a.Length-i)< (a.Length-i0)
+	modifies a
+	{
+		j,i,x,y:=j0,i0,x0,y0;
+		if a[j+2]!=x{
+		SwapPair(a,j+2,j+1,A);
+	}	
+	else{
+		LemmaMidNoswap(a[..],j,i,x,y,A);
+	}
+	
+	
+	while j>=0 && a[j] > y
+		invariant Inv3Pair(a[..],j,i,x,y,A)
+		decreases j
+		{
+			SwapPair(a,j+1,j,A);
+			j:=j-1;
+		}
+	
+	i:=i+2;	
+	}
 predicate method GuardMainLoop(a: array<int>,i:nat)
 {
 	i < a.Length-1	
+}
+
+predicate method GuardSecondLoop(a: array<int>,j:int,x:int)
+	requires -1<=j<=a.Length-3
+	reads a
+{
+	 j>=0 && a[j]>x	
+}
+
+
+lemma LemmaMidswap(a: seq<int>,j:int,i:nat,x:int,y:int, A: multiset<int>)
+	requires Inv2Pair(a,j,i,x,y,A)
+	requires j<0 || a[j]<=x
+	requires a[j+2]!=x
+	ensures Inv3Pair(a[j+1:=a[j+2]][j+2:=a[j+1]],j,i,x,y,A)
+{
+}
+
+lemma LemmaMidNoswap(a: seq<int>,j:int,i:nat,x:int,y:int, A: multiset<int>)
+	requires Inv2Pair(a,j,i,x,y,A)
+	requires j<0 || a[j]<=x
+	requires a[j+2]==x
+	ensures Inv3Pair(a,j,i,x,y,A)
+{
 }
 predicate InvPair(a: seq<int>, j: int, i:nat, A: multiset<int>)
 {
@@ -139,39 +251,6 @@ predicate Inv2Pair(a: seq<int>, j: int,i:nat,x:int, y:int, A: multiset<int>)
 	multiset(a)==A
 }
 
-
-
-lemma LemmaMidswap(a: seq<int>,j:int,i:nat,x:int,y:int, A: multiset<int>)
-	requires Inv2Pair(a,j,i,x,y,A)
-	requires j<0 || a[j]<=x
-	requires a[j+2]!=x
-	ensures Inv3Pair(a[j+1:=a[j+2]][j+2:=a[j+1]],j,i,x,y,A)
-{
-}
-
-lemma LemmaMidNoswap(a: seq<int>,j:int,i:nat,x:int,y:int, A: multiset<int>)
-	requires Inv2Pair(a,j,i,x,y,A)
-	requires j<0 || a[j]<=x
-	requires a[j+2]==x
-	ensures Inv3Pair(a,j,i,x,y,A)
-{
-}
-
-lemma firstLoop(a: seq<int>,j:int,i:nat,x:int,y:int, A: multiset<int>)
-	requires Inv2Pair(a,j,i,x,y,A) && j>=0 && a[j] > x
-	ensures Inv2Pair(a[j:=a[j+2]][j+2:=a[j]],j-1,i,x,y,A)
-{}
-lemma secondLoop(a: seq<int>,j:int,i:nat,x:int,y:int, A: multiset<int>)
-	requires Inv3Pair(a[..],j,i,x,y,A) && j>=0 && a[j] > y
-	ensures Inv3Pair(a[j:=a[j+1]][j+1:=a[j]],j-1,i,x,y,A)
-{}
-
-lemma fourthLoop(a: seq<int>,j:int,i:nat,x:int,y:int, A: multiset<int>)
-	requires Inv4Pair(a[..],j,i,x,y,A) && j>=0 && a[j] > y
-	ensures Inv4Pair(a[j:=a[j+1]][j+1:=a[j]],j-1,i,x,y,A)
-{
-}
-
 predicate Inv3Pair(a: seq<int>, j: int,i:nat,x:int, y:int, A: multiset<int>)
 {
 	0<=i<=|a|-2 &&
@@ -188,7 +267,7 @@ predicate Inv4Pair(a: seq<int>, j: int,i:nat,x:int, y:int, A: multiset<int>)
 {
 	-1<=j<=|a|-2&&
 	SortedSequence1(a,0,j)&&
-	SortedSequence1(a,j+2,|a|-1)&&
+	SortedSequence1(a,j+1,|a|-1)&&
 	a[j+1]==y && 
 	(j<=|a|-3 ==> a[j+2]>y) &&
 	(0<=j<=|a|-3 ==> a[j+2]>=a[j]) &&
@@ -203,9 +282,6 @@ predicate Sorted1(a: array<int>, i:nat, j:int)
 {
 	 (forall k :: i <= k < j-1 ==> a[k] <= a[k+1]) 
 }
-
-
-
 
 predicate SortedSequence1(a: seq<int>, i:nat, h:int)
 	requires i<=h ==> (0<=i <|a| && 0<=h<|a|)
@@ -238,3 +314,31 @@ lemma LemmaSwapPair(a: seq<int>,oldA :seq <int>, x: nat, y: nat, A: multiset<int
 	ensures  a[x:= oldA[y]][y:=oldA[x]][y] == oldA[x]
 	ensures forall i :: 0<=i<|a| ==> ((i!=x && i!=y) ==> a[x:= oldA[y]][y:=oldA[x]][i]==oldA[i])
 {}
+
+/*method {:verify true} SwapPair1(a: array<int>, x:nat,y:nat,i:nat,ghost A: multiset<int>)
+	requires multiset(a[..]) == A
+	requires 0<=x<a.Length && 0<=y<a.Length
+	requires 0<=i<=a.Length-2
+	requires SortedSequence1(a[..],0,x)&& SortedSequence1(a[..],y,i)
+	ensures multiset(a[..]) == A
+	ensures SortedSequence1(a[..],0,x) && SortedSequence1(a[..],y,i)
+	ensures 0<=i<=a.Length-2
+	modifies a
+{
+	// assignment
+	//LemmaSwapPair1(a[..],old(a[..]), x, y, A);
+	a[x], a[y] := a[y], a[x];
+}
+
+lemma LemmaSwapPair1(a: seq<int>,oldA :seq <int>, x: nat, y: nat, A: multiset<int>)
+	requires a==oldA
+	requires multiset(a[..]) == A
+	requires 0<=x<|a| && 0<=y<|a|
+	requires x!=y
+	ensures multiset(a[x:= oldA[y]][y:=oldA[x]]) == A
+	ensures a[x:= oldA[y]][y:=oldA[x]][x] == oldA[y]
+	ensures  a[x:= oldA[y]][y:=oldA[x]][y] == oldA[x]
+	ensures forall i :: 0<=i<|a| ==> ((i!=x && i!=y) ==> a[x:= oldA[y]][y:=oldA[x]][i]==oldA[i])
+{}
+
+*/
